New TypedAligned much better

TypeAligned.lean
@@ -1,133 +1,60 @@
 import Mathlib.Data.List.Basic
+import Pharoh.Queue
 
-namespace TypeAligned
+namespace List
 
-inductive List (arr : Type → Type → Type) : Type → Type → Type 2 where
-  | nil : List arr α α 
-  | cons : ∀ β, arr α β → List arr β γ → List arr α γ
+def TypeAligned {Ty} (dom cod : α → Ty) (τ σ : Ty) : List α → Prop
+  | []        => τ = σ
+  | (x :: xs) => τ = dom x ∧ TypeAligned dom cod (cod x) σ xs
 
-notation "[]" => List.nil
-infixr:60 "∷" => List.cons _
+@[simp]
+lemma TypeAligned_nil : ∀ {Ty} {dom cod : α → Ty} {τ σ}, TypeAligned dom cod τ σ [] = (τ = σ) := rfl
 
-open List
+@[simp]
+lemma TypeAligned_cons : ∀ {Ty} {dom cod : α → Ty} {τ σ} {x xs}, 
+  TypeAligned dom cod τ σ (x :: xs) = (τ = dom x ∧ TypeAligned dom cod (cod x) σ xs) := rfl
 
-instance (arr) (α : Type) : EmptyCollection (List arr α α) where
-  emptyCollection := nil
+@[simp]
+lemma TypeAligned_singleton : ∀ {Ty} {dom cod : α → Ty} {x}, 
+  TypeAligned dom cod (dom x) (cod x) [x] := by simp
 
-lemma empty_def (arr α) : (∅ : List arr α α) = [] := rfl
+lemma TypeAligned_append : ∀ {ls rs : List α} {τ σ ω : Ty},
+  ls.TypeAligned dom cod τ σ →
+  rs.TypeAligned dom cod σ ω →
+  (ls ++ rs).TypeAligned dom cod τ ω
+  | nil, rs, τ, σ, ω, l_TA, r_TA => by 
+    simp at *
+    cases l_TA
+    exact r_TA
+  | cons l ls, r, τ, σ, ω, l_TA, r_TA => by
+    simp at *
+    cases l_TA with | intro left right =>
+    apply (And.intro left)
+    apply TypeAligned_append
+    apply right
+    exact r_TA
 
-instance (arr) (α : Type) : EmptyCollection (List (flip arr) α α) where
-  emptyCollection := nil
-
-lemma empty_def' (arr α) : (∅ : List (flip arr) α α) = [] := rfl
-
-def hAppend {α β γ} (l : List arr α β) ( r : List arr β γ) : List arr α γ :=
-  match l with
-  | nil => r
-  | cons γ' l ls => l ∷ hAppend ls r
-
-instance : HAppend (List arr α β) (List arr β γ) (List arr α γ) where
-  hAppend := hAppend
-
-lemma nilAppend : ([] : List arr α α) ++ (x : List arr α β) = x := rfl
-lemma consAppend {α β β' γ} (r : List arr β γ) (x : arr α β') (xs : List arr β' β) : 
-  (cons β' x xs : List arr α β) ++ r = cons β' x (xs ++ r) := rfl
-
-lemma Iff.bothTrue : P → Q → (P ↔ Q) := 
-  λ p q => 
-    { mp  := fun h => q
-    , mpr := fun h => p 
-    }
-
-lemma Iff.bothFalse : ¬ P → ¬ Q → (P ↔ Q) := 
-  λ p q => 
-    { mp  := fun h => False.elim (p h)
-    , mpr := fun h => False.elim (q h) 
-    }
-
-lemma HEq.first {α β} {a : α} {b : β} : HEq a b → α = β
-  | HEq.refl _ => rfl
-
-lemma HEq.snd {a : α} {b : α} : HEq a b -> a = b
-  | HEq.refl _ => rfl
-
-lemma ConsNotHEqNil_aux : ¬ HEq (cons α' l ls : List arr α α) ([] : List arr α α) := by
-  simp
-
-lemma ConsNotHEqNil_aux2 : HEq (cons α' l ls : List arr α β) (x : List arr α α) → 
-  HEq (cons α' l ls : List arr α α) (x : List arr α α)
-  | HEq.refl _ => HEq.refl _
-
-lemma nilEqhAppend (α β) : ∀ (l : List arr α β) ( r : List arr β α), 
-  ∅ = (l ++ r) ↔ (α = β ∧ HEq l r ∧ HEq r (nil : List arr α α))
-  | nil, nil => by 
-    apply Iff.bothTrue (Eq.trans (rfl : ∅ = []) rfl)
-    repeat constructor
-  | nil, cons β' r rs => by
-    apply Iff.bothFalse
-    rw [nilAppend]
-    intros h
-    cases h
+lemma TypeAligned_reverse (l : List α) : ∀ {τ σ : Ty}, l.TypeAligned dom cod τ σ → l.reverse.TypeAligned cod dom σ τ := by
+  induction l with
+  | nil => apply Eq.symm
+  | cons x xs ih =>
     simp
-  | cons α' l ls, r => by
-    apply Iff.bothFalse
-    
-    rw [consAppend, empty_def]
-    intros h
-    cases h
-    
-    intros h
-    cases h with | intro αβ right => 
-    cases right with | intro lr rNil => 
-    have : HEq (cons α' l ls) ([] : List arr α α) := by
-      have test := HEq.first rNil
-      apply HEq.trans lr rNil
-    simp
+    intros τ σ α_eq_dom_x xs_typeAligned
+    apply TypeAligned_append (ih xs_typeAligned)
+    rw [α_eq_dom_x]
+    apply TypeAligned_singleton
+
+end List
+
+namespace Queue
+
+def TypeAligned {Ty} (dom cod : α → Ty) (τ σ : Ty) (q : Queue α) : Prop :=
+  ∃ ω : Ty, q.back.TypeAligned cod dom τ ω ∧ q.front.TypeAligned dom cod σ ω
+
+end Queue
 
 
-def reverseSpec : List arr α β → List (flip arr) β α
-  | nil => nil
-  | cons γ x xs => reverseSpec xs ++ (cons _ (x : flip arr γ α) nil : List (flip arr) _ _)
-
-def reverseEmpty (a : List arr α α) : reverseSpec a = ∅ ↔ (a = ∅) := 
-  Iff.intro 
-    ( λ h => by 
-      cases a with
-      | nil => rfl
-      | cons β x xs => 
-        have : reverseSpec (cons β x xs) = reverseSpec xs ++ (cons _ (x : flip arr β α) nil : List (flip arr) _ _)
-          := rfl
-        rw [this] at h
-    ) 
-    _
-
-inductive Queue (arr : Type → Type → Type) (α γ : Type) : Type 2 where 
-  | mk (β : Type) : List arr α β → List (flip arr) γ β → Queue arr α γ
-
-open Queue
-
-instance (arr) (α : Type) : EmptyCollection (Queue arr α α) where
-  emptyCollection := Queue.mk α nil nil
-
-def enqueue (x : arr α β) : Queue arr β γ → Queue arr α γ
-  | mk γ' back front => mk γ' (x ∷ back) front
-
-def dequeue :
-  ∀ (deque : Queue arr α γ),
-  (Σ β, Queue arr α β × arr β γ ) ⊕' (α = γ ∧ HEq deque (∅ : Queue arr α α)) := by
-  intros deque
-  cases deque with
-  | mk γ' back front =>
-    cases front with
-    | nil =>
-      cases reverseSpec back with
-      | nil =>
-        apply PSum.inr
-        simp
-        
 
 
-    | cons _ front middle =>
-      apply PSum.inl
-      exact (Sigma.mk _ (mk γ' back middle, front))
+
 
