lakefile.lean
@@ -1,7 +1,7 @@
 import Lake
 open System Lake DSL
 
-package pharoh {
+package Pharoh {
 dependencies := #[
     { name := `mathlib, src := Source.path (FilePath.mk "/home" / "nolrai" / "Lean4" / "mathlib4") }
    ]
